src/CompilationUnit.v
@@ -1,4 +1,4 @@
-Require Import List String HList SourceLang.
+Require Import List String HList SourceLifted.
 Import ListNotations.
 Require Semantics.
 Require Import HighValues.
@@ -6,30 +6,33 @@ Require Import Utopia.
 
 Record compilation_unit :=
   CompilationUnit {
-      types : list type;
-      exprs : hlist (expr []) types;
+      types : list (type * list type * type);
+      exprs : genv types;
        names : list string (* invariant: no duplicates and same length as types *)
   }.
 
-Definition singleton {ty} (e : expr [] ty) (name : string) : compilation_unit :=
-  CompilationUnit [ty] (hcons e hnil) [name].
+Definition singleton {ty} (e : body_expr [] ty) (name : string) : compilation_unit :=
+  CompilationUnit [ty] (GenvCons e GenvNil) [name].
 
-(* Initial state stuff for SourceLang *)
+(* Initial state stuff for SourceLifted *)
 
+(*
 (* Not sure how to write all the dependent types for this *)
-Inductive is_callstate (cu : compilation_unit) : forall tys ty, expr tys ty -> expr tys ty -> expr tys ty -> Prop := .
+Inductive is_callstate (cu : compilation_unit) :
+    forall G L ty, expr G L ty -> expr G L ty -> expr G L ty -> Prop := .
 (* | initial_intro :
     forall ty expr (m : member ty (types cu)),
       hget (exprs cu) m = expr ->
       initial_state cu nil ty expr.*)
 
 
-Inductive final_state (cu : compilation_unit) : forall tys ty, expr tys ty -> expr tys ty -> Prop :=
+Inductive final_state (cu : compilation_unit) :
+    forall G L ty, expr G L ty -> expr G L ty -> Prop :=
 | final_intr :
     forall ty expr,
-      SourceLang.value expr ->
+      SourceLifted.value expr ->
       final_state cu nil ty expr expr.
-      
+
 Definition source_semantics {ty : type} (cu : compilation_unit) : Semantics.semantics :=
   @Semantics.Semantics_gen (@SourceLang.expr nil ty) unit
                            (@SourceLang.expr nil ty)
@@ -39,3 +42,4 @@ Definition source_semantics {ty : type} (cu : compilation_unit) : Semantics.sema
                            (tt).
 
 
+*)
